\documentclass{article}
\usepackage{amsmath}

\title{Discrete 1}
\author{EE23BTECH11037-M.Esha}
\date{}

\begin{document}

\maketitle
\textbf{11.9.3.11-} Evaluate 
\[
\sum_{k=1}^{11} (2 + 3^k)
\]

The expression for \(x(n)\) is given by:
\[
x(n) = 2(n+1) + \frac{3^{n+1} - 1}{2} \quad \text{where} \ n=0,1,2,...
\]

The solution of the summation
\[
\sum_{k=1}^{11} (2 + 3^k)
\]
is
\[
x(11) - x(0) = \left[2(12) + \frac{3^{12} - 1}{2}\right] - \left[2(1) + \frac{3^{1} - 1}{2}\right]
\]

Simplifying further:
\[
x(11) - x(0) = 24 + \frac{3^{12} - 1}{2} - \left[2(1) + 1\right]
\]
\[
= 24 + \frac{3^{12} - 1}{2} - 3
\]
\[
= 21+ \frac{3^{12} - 1}{2}
\]


\end{document}

